% available style: report
\documentclass[12pt]{article}

\input{preamble}

\title{Complex Variable}
\author{Harry}
\date{\today}
\begin{document}
\section{Q3}
We are to prove that there is no $z \in \mathbb{C}$ such that $|z| = |z-2(1-i)| = 1$.

Let us invoke triangular-inequality:

$$
|z-2(1-i)| \geq	||z| - |2(1-i)|| = 2\sqrt{2} - 1 > 1
$$

This is a contradiction and we conclude that there is no such $z$.

\section{Q4}
I claim that all $z$ such that $|Re(z)| + |Im(z)| = \sqrt{2} |z|$ are $r e^{i \pi/4}$ and $r e^{i 3\pi/4}$ for any $r \in \bb{R}$.

Backword diretion: easy to verify with computation.

Forward direction:

For any $z = re^{i \theta}$, our constrains gives us: $|\sin{\theta}| + |\cos{\theta}| = \sqrt{2}$.

Consider the following cases:

$\sin{\theta} + \cos{\theta} = \sqrt{2}$. 
Notice $\sin{\theta} + \cos{\theta} = \sqrt{2}\sin{(\frac{\pi}{4} + \theta)} = \sqrt{2}$. (Apply identity for $\sin(a+b)$)
It is clear that the equaility is only established with $\theta = \frac{\pi}{4}$ for $0\leq \theta \leq 2\pi$.

Similarly, for 
$-\sin{\theta}  -\cos{\theta} = \sqrt{2}$, we can assert the equality is only established with $\theta = \frac{5\pi}{4}$ for $0\leq \theta \leq 2\pi$.


For $-\sin{\theta} + \cos{\theta} = \sqrt{2}$. We have
$-\sin{\theta} + \cos{\theta} = \sqrt{2}\sin{(\frac{3\pi}{4} + \theta)} = \sqrt{2}$. 
It is clear that the equaility is only established with $\theta = \frac{7\pi}{4}$ for $0\leq \theta \leq 2\pi$.

And for $\sin{\theta} - \cos{\theta} = \sqrt{2}$, the equality is only established with $\theta = \frac{3\pi}{4}$.

Note for all four cases we have set no restrain for $r$. 

Thus we conclude that all $z$ such that $|Re(z)| + |Im(z)| = \sqrt{2} |z|$ are $r e^{i \pi/4}$ and $r e^{i 3\pi/4}$ for any $r \in \bb{R}$.

\section{Q5}

I claim that, for all $\alpha>0$, we have $\frac{|z-\alpha|}{|z+\alpha|} < 1$ iff $Re(z) > 0$.

Let us write $z = a+ bi$ and $|z|^2 = a^2 + b^2$.

Again, there are three cases:

1): $a=0$.
In such case we have $(\frac{|z-\alpha|^2}{|z+\alpha|^2}) = (\frac{\alpha^2 + b^2}{\alpha^2 + b^2}) = 1$. As modular is always positive, we conclude that $\frac{|z-\alpha|}{|z+\alpha|} = 1$

2): $a>0$. 
Since $a, \alpha>0$, it is clear that $|a-\alpha| < |a+\alpha| \implies (a-\alpha)^2 < (a+\alpha)^2 \implies (a-\alpha)^2 + b^2 < (a+\alpha)^2 + b^2$ thus
in such case we have $\frac{|z-\alpha|^2}{|z+\alpha|^2} = \frac{(a-\alpha)^2 + b^2}{(a+\alpha)^2 + b^2} < 1 \implies \frac{|z-\alpha|}{|z+\alpha|} < 1$ (as modular is positive). 

3): $a<0$.
Since $a<0, \alpha>0$, it is clear that $|a-\alpha| > |a+\alpha| \implies (a-\alpha)^2 > (a+\alpha)^2 \implies (a-\alpha)^2 + b^2 > (a+\alpha)^2 + b^2$ thus 
in such case we have $\frac{|z-\alpha|^2}{|z+\alpha|^2} = \frac{(a-\alpha)^2 + b^2}{(a+\alpha)^2 + b^2} > 1 \implies \frac{|z-\alpha|}{|z+\alpha|} > 1$.

Thus we conclude that, for all $\alpha>0$, we have $\frac{|z-\alpha|}{|z+\alpha|} < 1$ iff $Re(z) > 0$.

\section{Q6}
We have  $z = x+iy$ and $x>0$. I claim that for $\epsilon = \frac{x}{2}$, and $w $ such that $|w-z| < \epsilon$, we have $Re(w) > 0$.

Let us write $w = a+bi$. Notice $|w-z|<\epsilon \implies (a-x)^2 + (b-y)^2 < \epsilon^2 \implies (a-x)^2 < \epsilon^2 \implies |x-a| < \frac{x}{2} $. As $\frac{x}{2}>0$, apply definition of absolute value, we have $ \frac{x}{2}<a<\frac{3x}{2}$. As $x > 0$ we have $a>x>0$ as desired. 
\end{document} 
